Isabelle/TFGCasper.thy
@@ -15,12 +15,6 @@ locale GhostParams = Params +
   (* Definition 4.24: Previous block resolver *)
   and prev :: "block \<Rightarrow> block"
 
-(* Locale for proofs *)
-locale Ghost = GhostParams + Protocol +
-  assumes prev_type : "\<forall> b. b \<in> B \<longleftrightarrow> prev b \<in> B"
-  and block_is_consensus_value : "B = C"
-  and ghost_is_estimator : "\<epsilon> = estimator"
-
 (* Definition 4.25: n'th generation ancestor block *)
 fun (in GhostParams) n_cestor :: "block * nat \<Rightarrow> block"
   where
@@ -44,10 +38,6 @@ fun (in GhostParams) score :: "state \<Rightarrow> block \<Rightarrow> real"
 fun (in GhostParams) children :: "block * state \<Rightarrow> block set"
   where
     "children (b, \<sigma>) = {b' \<in> est `\<sigma>. b = prev b'}"
-
-lemma (in Ghost) children_type :
-  "\<forall> b \<sigma>. b \<in> B \<and> \<sigma> \<in> \<Sigma> \<longrightarrow>  children (b, \<sigma>) \<subseteq> B"
-  using Ghost_axioms Ghost_axioms_def Ghost_def by auto
 
 (* Definition 4.29: Best Children *)
 fun (in GhostParams) best_children :: "block * state \<Rightarrow>  block set"
@@ -73,10 +63,28 @@ abbreviation (in GhostParams) P :: "consensus_value_property set"
   where
     "P \<equiv> {p. \<exists>!b \<in> B. \<forall>b' \<in> B. (b \<downharpoonright> b' \<longrightarrow> p b' = True) \<and> \<not> (b \<downharpoonright> b' \<longrightarrow> p b' = False)}"
 
+
+lemma (in GhostParams) GHOST_is_valid_estimator : 
+  "(\<forall> b. b \<in> B \<longleftrightarrow> prev b \<in> B) \<and> B = C \<and> genesis \<in> C 
+  \<Longrightarrow> is_valid_estimator estimator"
+  apply simp
+  oops
+
+(* Locale for proofs *)
+locale Ghost = GhostParams + Protocol +
+  assumes prev_type : "\<forall> b. b \<in> B \<longleftrightarrow> prev b \<in> B"
+  and block_is_consensus_value : "B = C"
+  and ghost_is_estimator : "\<epsilon> = estimator"
+  and genesis_type : "genesis \<in> C"
+
+lemma (in Ghost) children_type :
+  "\<forall> b \<sigma>. b \<in> B \<and> \<sigma> \<in> \<Sigma> \<longrightarrow>  children (b, \<sigma>) \<subseteq> B"
+  using Ghost_axioms Ghost_axioms_def Ghost_def by auto
+
 lemma (in Ghost) block_membership_property_is_majority_driven :
   "\<forall> p \<in> P. is_majority_driven p"
   apply simp
-  by (metis DiffE Pow_iff \<epsilon>_type block_is_consensus_value is_majority_driven_def subsetCE)
+  by (metis DiffE Pow_iff is_valid_estimator_def \<epsilon>_type block_is_consensus_value is_majority_driven_def subsetCE)
 
 lemma (in Ghost) block_membership_property_is_max_driven :
   "\<forall> p \<in> P. is_max_driven p"
